feat: Removed duplicate lemma generation

src/main/equivalence/expression.scala
@@ -7,14 +7,14 @@ import equivalence.program.functionEquivalence
 private def lookup[A, B](data: List[(A, B)], key: A): B =
     data.find((a, _) => a == key).get._2
 
-def mergeBasicExpr(modelExpr: BasicExpr, modelFunc: Function, candidateExpr: BasicExpr, candidateFunc: Function)(using program: Program): (Map[String, Lemma], List[(String, String)], List[Stmt]) = 
+def mergeBasicExpr(currentLemmas: Map[String, Lemma], modelExpr: BasicExpr, modelFunc: Function, candidateExpr: BasicExpr, candidateFunc: Function)(using program: Program): (Map[String, Lemma], List[(String, String)], List[Stmt]) = 
     (modelExpr, candidateExpr) match {
         case (TrueFunctionCall(calledInModel, calledInModelArgs), TrueFunctionCall(calledInCandidate, calledInCandidateArgs))
             if calledInModel != modelFunc.name && calledInCandidate != candidateFunc.name && calledInModelArgs.map(_.length).sum == calledInCandidateArgs.map(_.length).sum => {
             // Generate Equivalence data for the called functions
             val funcCalledInModel = program.helperFunctions(calledInModel)
             val funcCalledInCandidate = program.helperFunctions(calledInCandidate)
-            val (lemma, helperLemmas, mapping) = functionEquivalence(funcCalledInModel, funcCalledInCandidate)
+            val (lemma, helperLemmas, mapping) = functionEquivalence(currentLemmas, funcCalledInModel, funcCalledInCandidate)
 
             // Convert mapping between the parameters of the called functions to a mapping to the parameters in
             // the caller functions
@@ -30,9 +30,9 @@ def mergeBasicExpr(modelExpr: BasicExpr, modelFunc: Function, candidateExpr: Bas
             (helperLemmas + lemma, finalMapping, List(finalStmt))
         }
         case (Cond(modelCond, modelThen, modelElse), Cond(candidateCond, candidateThen, candidateElse)) => {
-            val (condHelpers, condMappings, condStmts) = mergeBasicExpr(modelCond, modelFunc, candidateCond, candidateFunc)
-            val (thenHelpers, thenMappings, thenStmts) = mergeExprBlock(modelThen, modelFunc, candidateThen, candidateFunc)
-            val (elseHelpers, elseMappings, elseStmts) = mergeExprBlock(modelElse, modelFunc, candidateElse, candidateFunc)
+            val (condLemmas, condMappings, condStmts) = mergeBasicExpr(currentLemmas, modelCond, modelFunc, candidateCond, candidateFunc)
+            val (thenLemmas, thenMappings, thenStmts) = mergeExprBlock(condLemmas, modelThen, modelFunc, candidateThen, candidateFunc)
+            val (elseLemmas, elseMappings, elseStmts) = mergeExprBlock(thenLemmas, modelElse, modelFunc, candidateElse, candidateFunc)
 
             val finalStmts = (thenStmts, elseStmts) match {
                 case (Nil, Nil) => condStmts
@@ -40,32 +40,32 @@ def mergeBasicExpr(modelExpr: BasicExpr, modelFunc: Function, candidateExpr: Bas
             }
 
             // TODO: Mappings concatenation
-            (condHelpers ++ thenHelpers ++ elseHelpers, condMappings ++ thenMappings ++ elseMappings, finalStmts)
+            (elseLemmas, condMappings ++ thenMappings ++ elseMappings, finalStmts)
         }
         case (Tuple(modelElements), Tuple(candElements)) if modelElements.length == candElements.length => {
-            val data = modelElements.zip(candElements).map((modelElem, candElem) => mergeBasicExpr(modelElem, modelFunc, candElem, candidateFunc))
-            data.foldLeft((Map(), List(), List())) {
-                case ((accHelpers, accMappings, accStmts), (helpers, mappings, stmts)) => (
-                    accHelpers ++ helpers, accMappings ++ mappings, accStmts ++ stmts
-                )
+            modelElements.zip(candElements).foldLeft((currentLemmas, Nil, Nil)) {
+                case ((accLemmas, accMappings, accStmts), (modelElem, candElem)) => {
+                    val (lemmas, mappings, stmts) = mergeBasicExpr(accLemmas, modelElem, modelFunc, candElem, candidateFunc)
+                    (lemmas, accMappings ++ mappings, accStmts ++ stmts)
+                }
             }
         }
         case (Binary(modelOp, modelLeft, modelRight), Binary(candOp, candLeft, candRight)) if modelOp == candOp => {
-            val (leftLemmas, leftMappings, leftStmts) = mergeBasicExpr(modelLeft, modelFunc, candLeft, candidateFunc)
-            val (rightLemmas, rightMappings, rightStmts) = mergeBasicExpr(modelRight, modelFunc, candRight, candidateFunc)
-            (leftLemmas ++ rightLemmas, leftMappings ++ rightMappings, leftStmts ++ rightStmts)
+            val (leftLemmas, leftMappings, leftStmts) = mergeBasicExpr(currentLemmas, modelLeft, modelFunc, candLeft, candidateFunc)
+            val (rightLemmas, rightMappings, rightStmts) = mergeBasicExpr(leftLemmas, modelRight, modelFunc, candRight, candidateFunc)
+            (rightLemmas, leftMappings ++ rightMappings, leftStmts ++ rightStmts)
         }
         case (Ident(modelName, Nil), Ident(candName, Nil)) => {
-            (Map(), List(modelName -> candName), Nil)
+            (currentLemmas, List(modelName -> candName), Nil)
         }
-        case _ => (Map(), Nil, Nil)
+        case _ => (currentLemmas, Nil, Nil)
     }
 
-def mergeExprBlock(modelExprBlock: ExprBlock, modelFunc: Function, candidateExprBlock: ExprBlock, candidateFunc: Function)(using program: Program): (Map[String, Lemma], List[(String, String)], List[Stmt]) = {
+def mergeExprBlock(currentLemmas: Map[String, Lemma], modelExprBlock: ExprBlock, modelFunc: Function, candidateExprBlock: ExprBlock, candidateFunc: Function)(using program: Program): (Map[String, Lemma], List[(String, String)], List[Stmt]) = {
     val ExprBlock(modelExtended, modelBasic) = modelExprBlock
     val ExprBlock(_, candBasic) = candidateExprBlock
 
-    val (lemmas, mappings, stmts) = mergeBasicExpr(modelBasic, modelFunc, candBasic, candidateFunc)
+    val (lemmas, mappings, stmts) = mergeBasicExpr(currentLemmas, modelBasic, modelFunc, candBasic, candidateFunc)
 
     val modelVariables = stmts match {
         case Nil => Nil
@@ -77,9 +77,9 @@ def mergeExprBlock(modelExprBlock: ExprBlock, modelFunc: Function, candidateExpr
     (lemmas, mappings, modelVariables ++ stmts)
 }
 
-def mergeFunction(modelFunc: Function, candidateFunc: Function)(using program: Program): (Map[String, Lemma], List[(String, String)], List[Stmt]) = {
+def mergeFunction(currentLemmas: Map[String, Lemma], modelFunc: Function, candidateFunc: Function)(using program: Program): (Map[String, Lemma], List[(String, String)], List[Stmt]) = {
     // Mappings are generated through merging the function bodys and through type matching
-    val (lemmas, mappings, stmts) = mergeExprBlock(modelFunc.body, modelFunc, candidateFunc.body, candidateFunc)
+    val (lemmas, mappings, stmts) = mergeExprBlock(currentLemmas, modelFunc.body, modelFunc, candidateFunc.body, candidateFunc)
 
     // Find parameters not covered by function body merging
     val modelParamsCovered = mappings.map(_._1)
