src/test/output/arrayHeap.dfy
@@ -2,18 +2,18 @@ function childrenAreHeapsM(a: seq<int>, N: int, i: int): bool
 requires ((((i >= 0) && (i < N)) && (N <= |a|)) && (N <= 100000))
 {var l := leftM(i);
 var r := rightM(i);
-if ((l < N) && (r < N)) then (isHeapM(a, N, l) && isHeapM(a, N, r)) else (!(l < N) || isHeapM(a, N, l))}
+if ((l < N) && (r < N)) then (isHeapM(a, N, l) && isHeapM(a, N, r)) else if (l < N) then isHeapM(a, N, l) else true}
 
 function childrenAreHeaps(a: seq<int>, N: int, i: int): bool
 requires ((((i >= 0) && (i < N)) && (N <= |a|)) && (N <= 100000))
-{if ((((2 * i) + 1) < N) && (((2 * i) + 2) < N)) then (isHeap(a, N, ((2 * i) + 1)) && isHeap(a, N, ((2 * i) + 2))) else (!(((2 * i) + 1) < N) || isHeap(a, N, ((2 * i) + 1)))}
+{if ((((2 * i) + 1) < N) && (((2 * i) + 2) < N)) then (isHeap(a, N, ((2 * i) + 1)) && isHeap(a, N, ((2 * i) + 2))) else if (((2 * i) + 1) < N) then isHeap(a, N, ((2 * i) + 1)) else true}
 
 function isHeap(a: seq<int>, N: int, i: int): bool
 requires ((((i >= 0) && (i < N)) && (N <= |a|)) && (N <= 100000))
 decreases ((N - i))
 {var l := ((2 * i) + 1);
 var r := ((2 * i) + 2);
-(!((((2 * i) + 1) < N) && (a[((2 * i) + 1)] > a[i])) && (!((((2 * i) + 2) < N) && (a[r] > a[i])) && if (((2 * i) + 2) < i) then (isHeap(a, N, ((2 * i) + 2)) && isHeap(a, N, ((2 * i) + 1))) else (!(((2 * i) + 1) < i) || isHeap(a, N, ((2 * i) + 1)))))}
+(!((((2 * i) + 1) < N) && (a[((2 * i) + 1)] > a[i])) && (!((((2 * i) + 2) < N) && (a[r] > a[i])) && if (((2 * i) + 2) < i) then (isHeap(a, N, ((2 * i) + 2)) && isHeap(a, N, ((2 * i) + 1))) else if (((2 * i) + 1) < i) then isHeap(a, N, ((2 * i) + 1)) else true))}
 
 function rightM(i: int): int
 requires ((0 <= i) && (i < 100000))
@@ -30,12 +30,12 @@ decreases ((N - i))
 var r := rightM(i);
 var isHeapL := ((l < N) && isHeapM(a, N, l));
 var isHeapR := ((r < N) && isHeapM(a, N, r));
-(!((l < N) && (a[l] > a[i])) && (!((r < N) && (a[r] > a[i])) && if (r < i) then (isHeapL && isHeapR) else (!(l < i) || isHeapL)))}
+(!((l < N) && (a[l] > a[i])) && (!((r < N) && (a[r] > a[i])) && if (r < i) then (isHeapL && isHeapR) else if (l < i) then isHeapL else true))}
 
 lemma childrenAreHeapsM_childrenAreHeaps_Equivalence(a: seq<int>, N: int, i: int)
 requires ((((i >= 0) && (i < N)) && (N <= |a|)) && (N <= 100000))
 ensures (childrenAreHeapsM(a, N, i) == childrenAreHeaps(a, N, i))
-{{var l := leftM(i);var r := rightM(i);if ((l < N) && (r < N)){isHeapM_isHeap_Equivalence(a, N, l);isHeapM_isHeap_Equivalence(a, N, r);}else {isHeapM_isHeap_Equivalence(a, N, l);}}}
+{{var l := leftM(i);var r := rightM(i);if ((l < N) && (r < N)){isHeapM_isHeap_Equivalence(a, N, l);isHeapM_isHeap_Equivalence(a, N, r);}else {if (l < N){isHeapM_isHeap_Equivalence(a, N, l);}else {}}}}
 
 lemma isHeapM_isHeap_Equivalence(a: seq<int>, N: int, i: int)
 requires ((((i >= 0) && (i < N)) && (N <= |a|)) && (N <= 100000))
